Complete all interesting cases

meta-theory/pure_letrecScript.sml
@@ -14,6 +14,9 @@ val _ = new_theory "pure_letrec";
 Inductive letrec_binds:
 [~swap:]
   (∀b1 b2 x y.
+    MAP FST b1 = MAP FST b2 ∧
+    EVERY (λe. freevars e ⊆ set (MAP FST b1)) (MAP SND b1) ∧
+    EVERY (λe. freevars e ⊆ set (MAP FST b2)) (MAP SND b2) ∧
     letrec_binds b1 b2 x y ⇒
     letrec_binds b1 b2 (Letrec b1 x) (Letrec b2 y)) ∧
   (* cases below are just recursion *)
@@ -65,6 +68,189 @@ Proof
   \\ imp_res_tac LIST_REL_opp \\ fs [SF ETA_ss]
 QED
 
+Theorem letrec_binds_freevars:
+  ∀b1 b2 x y. letrec_binds b1 b2 x y ⇒ freevars x = freevars y
+Proof
+  Induct_on ‘letrec_binds’ \\ rw [] \\ gvs []
+  >- (fs [EXTENSION,EVERY_MEM,MEM_MAP,PULL_EXISTS,EXISTS_PROD,FORALL_PROD,SUBSET_DEF]
+      \\ metis_tac [])
+  >- (pop_assum mp_tac
+      \\ qid_spec_tac ‘xs’
+      \\ qid_spec_tac ‘ys’
+      \\ Induct \\ Cases_on ‘xs’ \\ fs [])
+  \\ last_x_assum mp_tac
+  \\ qid_spec_tac ‘xs’
+  \\ qid_spec_tac ‘ys’
+  \\ Induct \\ fs []
+  \\ fs [PULL_EXISTS]
+  \\ strip_tac \\ Cases \\ fs []
+  \\ strip_tac \\ res_tac \\ fs [UNCURRY]
+  \\ gvs [EXTENSION]
+  \\ metis_tac []
+QED
+
+Theorem subst_exp_eq:
+  ∀y m1 m2 b.
+    FDOM m1 = FDOM m2 ∧
+    (∀k v1 v2. FLOOKUP m1 k = SOME v1 ∧ FLOOKUP m2 k = SOME v2 ⇒ (v1 ≃ v2) b) ⇒
+    (subst m1 y ≅? subst m2 y) b
+Proof
+  ho_match_mp_tac freevars_ind \\ rw []
+  >-
+   (fs [subst_def] \\ rpt CASE_TAC
+    \\ fs [exp_eq_refl]
+    \\ res_tac \\ fs [app_bisimilarity_eq]
+    \\ gvs [FLOOKUP_DEF])
+  >-
+   (fs [subst_def,SF ETA_ss]
+    \\ irule exp_eq_Prim_cong
+    \\ last_x_assum mp_tac
+    \\ qid_spec_tac ‘es’ \\ Induct
+    \\ fs [SF DNF_ss]
+    \\ metis_tac [])
+  >-
+   (fs [subst_def,SF ETA_ss]
+    \\ irule exp_eq_App_cong
+    \\ metis_tac [])
+  >-
+   (fs [subst_def,SF ETA_ss]
+    \\ irule exp_eq_Lam_cong
+    \\ last_x_assum irule
+    \\ fs [DOMSUB_FLOOKUP_THM,AllCaseEqs()]
+    \\ rw [] \\ res_tac \\ fs [])
+  \\ fs [subst_def,SF ETA_ss]
+  \\ irule exp_eq_Letrec_cong
+  \\ fs [MAP_MAP_o,combinTheory.o_DEF,UNCURRY]
+  \\ first_x_assum $ irule_at Any
+  \\ fs [FDOM_FDIFF,EXTENSION,FLOOKUP_FDIFF]
+  \\ rw [] \\ res_tac \\ fs []
+  \\ last_x_assum mp_tac
+  \\ last_x_assum mp_tac
+  \\ last_x_assum mp_tac
+  \\ qid_spec_tac ‘m2’
+  \\ qid_spec_tac ‘m1’
+  \\ qid_spec_tac ‘lcs’
+  \\ Induct
+  \\ fs [SF DNF_ss,FORALL_PROD]
+  \\ rw []
+  >-
+   (pop_assum kall_tac
+    \\ first_x_assum irule
+    \\ fs [FDOM_FDIFF,EXTENSION,FLOOKUP_FDIFF]
+    \\ metis_tac [])
+  \\ rewrite_tac [GSYM finite_mapTheory.FDIFF_FDOMSUB_INSERT]
+  \\ first_x_assum irule
+  \\ fs [FDOM_FDIFF,EXTENSION,FLOOKUP_FDIFF]
+  \\ fs [DOMSUB_FLOOKUP_THM,AllCaseEqs()]
+  \\ metis_tac []
+QED
+
+Triviality MAP_ID:
+  ∀xs f. (MAP f xs = xs) ⇔ ∀x. MEM x xs ⇒ f x = x
+Proof
+  Induct \\ fs [] \\ metis_tac []
+QED
+
+Theorem subst_letrec_binds:
+  ∀b1 b2 x y m1 m2.
+    letrec_binds b1 b2 x y ∧
+    FDOM m1 = FDOM m2 ∧
+    FDOM m1 SUBSET set (MAP FST b1) ∧
+    MAP FST b1 = MAP FST b2 ∧
+    (∀k v1 v2.
+      FLOOKUP m1 k = SOME v1 ∧ FLOOKUP m2 k = SOME v2 ⇒
+      letrec_binds b1 b2 v1 v2) ⇒
+    letrec_binds b1 b2 (subst m1 x) (subst m2 y)
+Proof
+  Induct_on ‘letrec_binds’ \\ rw []
+  >-
+   (fs [subst_def]
+    \\ simp [Once letrec_binds_cases]
+    \\ disj1_tac
+    \\ fs [MAP_ID,FORALL_PROD]
+    \\ reverse (rw [])
+    >-
+     (last_x_assum irule \\ fs [FDOM_FDIFF,EXTENSION,SUBSET_DEF]
+      \\ fs [FDOM_FDIFF,EXTENSION,FLOOKUP_FDIFF]
+      \\ rw [] \\ res_tac \\ fs []
+      \\ metis_tac [])
+    \\ irule pure_exp_lemmasTheory.subst_ignore
+    \\ CCONTR_TAC \\ gvs [IN_DISJOINT,EVERY_MEM,SUBSET_DEF])
+  >-
+   (fs [subst_def] \\ rpt CASE_TAC \\ fs [letrec_binds_refl]
+    \\ res_tac \\ fs [] \\ gvs [FLOOKUP_DEF])
+  >-
+   (fs [subst_def]
+    \\ simp [Once letrec_binds_cases]
+    \\ last_x_assum irule \\ fs []
+    \\ fs [DOMSUB_FLOOKUP_THM,AllCaseEqs()]
+    \\ rw [] \\ res_tac \\ fs [SUBSET_DEF])
+  >-
+   (fs [subst_def]
+    \\ simp [Once letrec_binds_cases]
+    \\ rpt $ last_x_assum $ irule_at Any \\ fs [])
+  >-
+   (fs [subst_def]
+    \\ simp [Once letrec_binds_cases,SF ETA_ss]
+    \\ last_x_assum mp_tac \\ fs []
+    \\ qid_spec_tac ‘ys’
+    \\ qid_spec_tac ‘xs’
+    \\ Induct \\ fs [PULL_EXISTS]
+    \\ rw [] \\ metis_tac [])
+  >-
+   (fs [subst_def]
+    \\ simp [Once letrec_binds_cases] \\ disj2_tac
+    \\ fs [MAP_MAP_o,combinTheory.o_DEF,UNCURRY,SF ETA_ss]
+    \\ reverse conj_tac
+    >-
+     (last_x_assum irule
+      \\ fs [FDOM_FDIFF,EXTENSION,FLOOKUP_FDIFF,SUBSET_DEF]
+      \\ rw [] \\ res_tac \\ fs [])
+    \\ last_x_assum mp_tac
+    \\ last_x_assum mp_tac
+    \\ pop_assum mp_tac
+    \\ pop_assum mp_tac
+    \\ pop_assum mp_tac
+    \\ pop_assum mp_tac
+    \\ qid_spec_tac ‘m2’
+    \\ qid_spec_tac ‘m1’
+    \\ qid_spec_tac ‘ys’
+    \\ qid_spec_tac ‘xs’
+    \\ Induct \\ fs [PULL_EXISTS]
+    \\ strip_tac \\ Cases \\ fs []
+    \\ rw []
+    >-
+     (first_x_assum irule
+      \\ fs [FDOM_FDIFF,EXTENSION,FLOOKUP_FDIFF,SUBSET_DEF]
+      \\ rw [] \\ res_tac \\ fs [])
+    \\ rewrite_tac [GSYM finite_mapTheory.FDIFF_FDOMSUB_INSERT]
+    \\ first_x_assum irule
+    \\ fs [FDOM_FDIFF,EXTENSION,FLOOKUP_FDIFF]
+    \\ fs [DOMSUB_FLOOKUP_THM,AllCaseEqs(),SUBSET_DEF]
+    \\ rw [] \\ res_tac \\ fs [])
+QED
+
+Triviality FDOM_UPDATES_EQ:
+  ∀b1. FDOM (FEMPTY |++ MAP (λ(g,x). (g,Letrec b2 x)) b1) = set (MAP FST b1)
+Proof
+  fs [FDOM_FUPDATE_LIST,MAP_MAP_o,combinTheory.o_DEF,UNCURRY,SF ETA_ss]
+QED
+
+Triviality FORALL_FRANGE:
+  (∀v. v ∈ FRANGE m ⇒ P v) ⇔ ∀k v. FLOOKUP m k = SOME v ⇒ P v
+Proof
+  fs [FRANGE_DEF,FLOOKUP_DEF,PULL_EXISTS]
+QED
+
+Triviality MEM_IMP_EQ:
+  ∀b1 k p1 p2.
+    MEM (k,p1) b1 ∧ MEM (k,p2) b1 ∧ ALL_DISTINCT (MAP FST b1) ⇒ p1 = p2
+Proof
+  Induct \\ fs [FORALL_PROD] \\ rw []
+  \\ fs [MEM_MAP,EXISTS_PROD]
+  \\ res_tac \\ fs []
+QED
+
 Theorem eval_forward_letrec_binds:
   ALL_DISTINCT (MAP FST binds2) ∧
   MAP FST binds1 = MAP FST binds2 ∧
@@ -103,15 +289,71 @@ Proof
            combinTheory.o_DEF,UNCURRY,SF ETA_ss])
   \\ ‘(Letrec b2 y ≃ subst_funs b2 y) b’ by
    (irule eval_IMP_app_bisimilarity
-    \\ fs [eval_Letrec] \\ cheat)
+    \\ imp_res_tac letrec_binds_freevars
+    \\ fs [eval_Letrec]
+    \\ rw [subst_funs_def,bind_def]
+    \\ rpt $ irule_at Any IMP_closed_subst
+    \\ fs [FDOM_UPDATES_EQ,PULL_EXISTS,alistTheory.flookup_fupdate_list]
+    \\ fs [FORALL_FRANGE,alistTheory.flookup_fupdate_list,AllCaseEqs()]
+    \\ rw []
+    \\ imp_res_tac ALOOKUP_MEM
+    \\ gvs [EVERY_MEM] \\ res_tac \\ fs []
+    \\ fs [MEM_MAP,EXISTS_PROD,PULL_EXISTS,EVERY_MEM])
   \\ ‘∀e. (e ≃ e2) b ⇔ (e ≃ subst_funs b2 y) b’ by
     metis_tac [app_bisimilarity_trans,app_bisimilarity_sym]
   \\ fs []
   \\ simp [subst_funs_def,bind_def]
-  \\ reverse IF_CASES_TAC >- cheat
-  \\ reverse IF_CASES_TAC >- cheat
+  \\ reverse IF_CASES_TAC >-
+   (fs [FDOM_UPDATES_EQ,PULL_EXISTS,alistTheory.flookup_fupdate_list]
+    \\ gvs [AllCaseEqs()]
+    \\ imp_res_tac ALOOKUP_MEM
+    \\ gvs [EVERY_MEM] \\ res_tac \\ fs []
+    \\ gvs [MEM_MAP,EXISTS_PROD,PULL_EXISTS,EVERY_MEM]
+    \\ res_tac \\ fs [])
+  \\ reverse IF_CASES_TAC >-
+   (fs [FDOM_UPDATES_EQ,PULL_EXISTS,alistTheory.flookup_fupdate_list]
+    \\ gvs [AllCaseEqs()]
+    \\ imp_res_tac ALOOKUP_MEM
+    \\ gvs [EVERY_MEM] \\ res_tac \\ fs []
+    \\ gvs [MEM_MAP,EXISTS_PROD,PULL_EXISTS,EVERY_MEM]
+    \\ res_tac \\ fs [])
   \\ qexists_tac ‘subst (FEMPTY |++ MAP (λ(g,x). (g,Letrec b2 x)) b1) y’
-  \\ cheat
+  \\ simp [app_bisimilarity_eq]
+  \\ rpt $ irule_at Any IMP_closed_subst
+  \\ irule_at Any subst_letrec_binds
+  \\ irule_at Any subst_exp_eq
+  \\ imp_res_tac letrec_binds_freevars
+  \\ fs [FDOM_UPDATES_EQ,PULL_EXISTS,alistTheory.flookup_fupdate_list]
+  \\ fs [FORALL_FRANGE,alistTheory.flookup_fupdate_list,AllCaseEqs()]
+  \\ rw []
+  \\ imp_res_tac ALOOKUP_MEM
+  \\ gvs [EVERY_MEM] \\ res_tac \\ fs []
+  \\ fs [MEM_MAP,EXISTS_PROD,PULL_EXISTS,EVERY_MEM]
+  \\ res_tac \\ gvs []
+  >-
+   (rename [‘(ll _ ≃ _) _’]
+    \\ qpat_x_assum ‘LIST_REL _ _ _’ mp_tac
+    \\ qpat_x_assum ‘MEM _ b2’ mp_tac
+    \\ qpat_x_assum ‘MEM _ b1’ mp_tac
+    \\ last_x_assum mp_tac
+    \\ last_x_assum mp_tac
+    \\ rename [‘MEM (kk,p_2) b2 ⇒ MEM (kk,p_1) b1 ⇒ _’]
+    \\ qid_spec_tac ‘p_1’
+    \\ qid_spec_tac ‘p_2’
+    \\ qid_spec_tac ‘b1’
+    \\ qid_spec_tac ‘b2’
+    \\ Induct \\ fs [PULL_EXISTS,FORALL_PROD,SF DNF_ss]
+    \\ rw []
+    >- (fs [MEM_MAP,EXISTS_PROD] \\ gvs [])
+    \\ first_x_assum irule \\ fs []
+    \\ ‘MEM kk (MAP FST b2')’ by (simp_tac std_ss [MEM_MAP,EXISTS_PROD] \\ metis_tac [])
+    \\ gvs [] \\ metis_tac [])
+  \\ ‘p_2 = p_2'’ by metis_tac [MEM_IMP_EQ]
+  \\ rw []
+  \\ irule letrec_binds_swap
+  \\ fs []
+  \\ res_tac \\ fs [letrec_binds_refl]
+  \\ fs [EVERY_MEM,EXISTS_PROD,MEM_MAP]
 QED
 
 Theorem exp_eq_Letrec_change_lemma[local]:
@@ -156,10 +398,17 @@ Proof
   Induct \\ fs [PULL_EXISTS] \\ metis_tac []
 QED
 
+Triviality LIST_REL_IMP_same_keys:
+  ∀binds1 binds2.
+    LIST_REL (λ(v1,e1) (v2,e2). v1 = v2) binds1 binds2 ⇒
+    MAP FST binds1 = MAP FST binds2
+Proof
+  Induct \\ fs [PULL_EXISTS,FORALL_PROD]
+QED
+
 Theorem exp_eq_Letrec_change:
   ∀binds1 binds2 e b.
     ALL_DISTINCT (MAP FST binds1) ∧
-    MAP FST binds1 = MAP FST binds2 ∧
     LIST_REL (λ(v1, e1) (v2, e2).
       v1 = v2 ∧ (Letrec binds1 e1 ≅? Letrec binds1 e2) b) binds1 binds2 ∧
     LIST_REL (λ(v1, e1) (v2, e2).
@@ -168,6 +417,10 @@ Theorem exp_eq_Letrec_change:
     (Letrec binds1 e ≅? Letrec binds2 e) b
 Proof
   rw [exp_eq_def]
+  \\ ‘MAP FST binds1 = MAP FST binds2’ by
+   (irule LIST_REL_IMP_same_keys
+    \\ qpat_x_assum ‘LIST_REL _ _ _’ mp_tac
+    \\ match_mp_tac LIST_REL_mono \\ fs [FORALL_PROD])
   \\ ‘closed (bind f (Letrec binds1 e)) ∧
       closed (bind f (Letrec binds2 e))’ by
    (rw [] \\ irule pure_exp_lemmasTheory.IMP_closed_bind \\ fs [])
